Classes/Monad/MonadJoin.v
@@ -7,8 +7,18 @@ Class MonadJoin M {MM : Monad M} : Type := {
     mjoin (returnM x) (returnM y) = returnM (x ⊔ y);
 }.
 Hint Rewrite @mjoin_return : monads.
-
 Infix "<⊔>" := mjoin (at level 40).
+
+Class MonadJoinSound (M M' : Type → Type) {MM : Monad M} {MJ : MonadJoin M}
+  {MM' : Monad M'} {GM : ∀ A A', Galois A A' → Galois (M A) (M' A')} : Type :=
+{
+  mjoin_sound_left : ∀ {A A'} {JA : Joinable A A} {JAI : JoinableIdem JA} 
+    {GA : Galois A A'} {JS : JoinableSound JA} (m1 m2 : M A) (m' : M' A'),
+    γ m1 m' → γ (m1 <⊔> m2) m';
+  mjoin_sound_right : ∀ {A A'} {JA : Joinable A A} {JAI : JoinableIdem JA}
+    {GA : Galois A A'} {JS : JoinableSound JA} (m1 m2 : M A) (m' : M' A'),
+    γ m2 m' → γ (m1 <⊔> m2) m';
+}.
 
 Definition mjoin_option A {JA : Joinable A A} {JI : JoinableIdem JA} : 
   option A → option A → option A :=
@@ -23,3 +33,16 @@ Proof.
   split with mjoin_option. reflexivity.
 Defined.
 Hint Resolve option_monadjoin : soundness.
+
+Instance option_monadjoin_sound : MonadJoinSound option option.
+Proof.
+  constructor; intros.
+  - destruct m1, m2; try constructor. destruct m'.
+    + constructor. apply join_sound.  constructor. inversion H;subst.
+      apply H2.
+    + inversion H.
+  - destruct m1, m2; try constructor. destruct m'.
+    + constructor. apply join_sound. right. inversion H; subst.
+      apply H2.
+    + inversion H. 
+Qed.
