Soundness.v
@@ -234,10 +234,9 @@ Theorem sound_interpreter: ∀ c,
     (boolType:=bool) (natType:=nat) c).
 Proof.
   eapply shared_ceval_sound; eauto 10 with soundness. 
-  - admit.
-  - admit.
-  - admit.
-  - apply if_top_sound. eauto 10 with soundness. 
+  apply catch_optionAT_sound; eauto with soundness.
+  apply stateT_monadjoin_sound.
+  apply if_top_sound. eauto 10 with soundness. 
   apply if_ab_op_sound. 
-Admitted.
+Qed.
 
